attempt on big code correctness lemma

WPDS/WAutomaton.thy
@@ -18,7 +18,7 @@ type_synonym ('state, 'label, 'weight) w_transition_set = "('state, ('label list
 definition wts_to_monoidLTS :: "('state, 'label, 'weight::bounded_idempotent_semiring) w_transitions \<Rightarrow> ('state, ('label list \<times> 'weight)) transition set" where
   "wts_to_monoidLTS ts = {(p, ([l],d), q) | p l d q. ts $ (p,l,q) = d}"
 
-definition wts_to_weightLTS :: "('state, 'label, 'weight::bounded_idempotent_semiring) w_transitions \<Rightarrow> ('state, 'weight) transition set" where
+definition wts_to_weightLTS :: "('state::finite, 'label::finite, 'weight::bounded_idempotent_semiring) w_transitions \<Rightarrow> ('state, 'weight) transition set" where
   "wts_to_weightLTS ts = {(p, d, q) | p l d q. ts $ (p,l,q) = d}"
 
 lemma "finite (wts_to_weightLTS ts)" oops (* THIS should be true!! *)
